theories/simulations/msim/ISim.v
@@ -821,7 +821,7 @@ End SIM.
 
 Global Opaque isim.
 
-Section Proph.
+Section FancyReal.
 
   Context `{Σ: GRA}.
 
@@ -837,19 +837,18 @@ Section Proph.
   Context (st_s st_t : alist key Any.t).
 
   (* Precise Pre & Post conditions *)
-  Lemma isim_update_proph_src_advanced {X A R} pre (post : X → R → iProp Σ) (arg : A) r g k_s i_t :
-    (∃ (I P : iProp Σ) (ret : R),
+  Lemma isim_fr_prepost_src_advanced {X} (pre post : X → _) r g k_s i_t :
+    (∃ (I P : iProp Σ),
       I ∗ precise P ∗
-      (∀ x, ∃ T, (I ∗ pre x arg -∗ □ T) ∗ (□ T -∗ pre x arg ==∗ P ∗ post x ret)) ∗
-      (P ∗ I ==∗ isim r g RR true pt (st_s, k_s ret) (st_t, i_t))) ⊢
-    isim r g RR ps pt (st_s, UpdateProph pre post arg >>= k_s) (st_t, i_t).
+      (∀ x, ∃ T, (I ∗ pre x -∗ □ T) ∗ (□ T -∗ pre x ==∗ P ∗ post x)) ∗
+      (P ∗ I ==∗ isim r g RR true pt (st_s, k_s ()) (st_t, i_t))) ⊢
+    isim r g RR ps pt (st_s, FRPrePost pre post >>= k_s) (st_t, i_t).
   Proof using.
-    iIntros "[%I [%P [%ret [I [#[%pr Pre] [Hsplit Hsim]]]]]]".
+    iIntros "[%I [%P [I [#[%pr Pre] [Hsplit Hsim]]]]]".
     iRevert "Hsplit Hsim Pre"; iStopProof.
     eapply entails_pointwise; iIntros (res Hres) "I Hsplit Hsim #[Hpre1 Hpre2]".
-    rewrite /UpdateProph; unseal CRIS_PROPH.
+    rewrite /FRPrePost; unseal CRIS_FancyReal.
     norm_l; iApply isim_choose_src; iExists (pr ⋅ res).
-    norm_l; iApply isim_choose_src; iExists ret.
     norm_l; iApply isim_guarantee_src; iSplitL "I Hsplit".
     { iIntros (x) "Pre"; iPoseProof ("Hsplit" $! x) as "[%T [HT Hsplit]]".
       iPoseProof ("HT" with "[I Pre]") as "#T".
@@ -863,16 +862,16 @@ Section Proph.
     norm_l; iMod ("Hsim" with "[P R]") as "$"; iFrame; iApply "Hpre1".
   Qed.
 
-  Lemma isim_update_proph_src {X A R} pre (post : X → R → iProp Σ) (arg : A) r g k_s i_t :
-    (∃ (P : iProp Σ) (ret : R),
+  Lemma isim_fr_prepost_src {X} (pre post : X → _) r g k_s i_t :
+    (∃ (P : iProp Σ),
       precise P ∗
-      (∀ x, pre x arg ==∗ P ∗ post x ret) ∗
-      (P ==∗ isim r g RR true pt (st_s, k_s ret) (st_t, i_t))) ⊢
-    isim r g RR ps pt (st_s, UpdateProph pre post arg >>= k_s) (st_t, i_t).
+      (∀ x, pre x ==∗ P ∗ post x) ∗
+      (P ==∗ isim r g RR true pt (st_s, k_s ()) (st_t, i_t))) ⊢
+    isim r g RR ps pt (st_s, FRPrePost pre post >>= k_s) (st_t, i_t).
   Proof using.
-    iIntros "[%P [%ret [Hprecise [Hsplit Hsim]]]]".
-    iApply isim_update_proph_src_advanced.
-    iExists True%I, P, ret.
+    iIntros "[%P [Hprecise [Hsplit Hsim]]]".
+    iApply isim_fr_prepost_src_advanced.
+    iExists True%I, P.
     iSplit; [done|iSplit; [done|]].
     iSplitL "Hsplit".
     { iIntros (?); iExists emp%I; iSplitR; [iIntros "_"; done|].
@@ -881,46 +880,44 @@ Section Proph.
     by iIntros "[P _]"; iApply "Hsim".
   Qed.
 
-  Lemma isim_update_proph_tgt {X A R} pre (post : X → R → iProp Σ) (arg : A) r g k_t i_s :
-    (∃ x, pre x arg ∗
-      ∀ ret, post x ret -∗ isim r g RR ps true (st_s, i_s) (st_t, k_t ret)) ⊢
-    isim r g RR ps pt (st_s, i_s) (st_t, UpdateProph pre post arg >>= k_t).
+  Lemma isim_fr_prepost_tgt {X} (pre post : X → _) r g i_s k_t :
+    (∃ x, pre x ∗ (post x -∗ isim r g RR ps true (st_s, i_s) (st_t, k_t ())))
+    ⊢
+    isim r g RR ps pt (st_s, i_s) (st_t, FRPrePost pre post >>= k_t).
   Proof using.
     iIntros "[%x [Hpre Hsim]]".
-    rewrite /UpdateProph; unseal CRIS_PROPH.
+    rewrite /FRPrePost; unseal CRIS_FancyReal.
     norm_r; iApply isim_choose_tgt; iIntros (pr).
-    (* norm_r; iApply isim_choose_tgt; iIntros (Q). *)
-    norm_r; iApply isim_choose_tgt; iIntros (ret).
     norm_r; iApply isim_guarantee_tgt; iIntros "P".
     iMod ("P" with "Hpre") as "[Hpr Hpost]".
     norm_r; iApply isim_assume_res_tgt; iFrame "Hpr".
-    (* norm_r; iApply isim_guarantee_tgt; iIntros "Q"; iMod ("Hpost" with "Q"). *)
     norm_r; iApply "Hsim"; done.
   Qed.
 
-  Lemma isim_update_proph_both
-      {X_s A_s R2_s X_t A_t R2_t}
-      (pre_s : X_s → A_s → iProp Σ) (post_s : X_s → R2_s → iProp Σ) (arg_s : A_s)
-      (pre_t : X_t → A_t → iProp Σ) (post_t : X_t → R2_t → iProp Σ) (arg_t : A_t)
-      r g k_s k_t :
-    (∀ ret_t P_t, precise P_t -∗
-      (∀ x, pre_t x arg_t ==∗ P_t ∗ post_t x ret_t) -∗
-      ∃ (P_s : iProp Σ) ret_s,
-        precise P_s ∗
-        (∀ x, pre_s x arg_s ==∗ P_s ∗ post_s x ret_s) ∗
-        (P_s ==∗ P_t ∗ isim r g RR true true (st_s, k_s ret_s) (st_t, k_t ret_t))) ⊢
+  Lemma isim_fr_prepost_both
+      {X_s X_t} r g
+      (pre_s post_s: X_s → _) (pre_t post_t: X_t → _)
+      k_s k_t
+    :
+    (∀ P_t,
+       precise P_t -∗
+       (∀ x, pre_t x ==∗ P_t ∗ post_t x) -∗
+       ∃ P_s,
+         precise P_s ∗
+         (∀ x, pre_s x ==∗ P_s ∗ post_s x) ∗
+         (P_s ==∗ P_t ∗ isim r g RR true true (st_s, k_s ()) (st_t, k_t ())))
+    ⊢
     isim r g RR ps pt
-      (st_s, UpdateProph pre_s post_s arg_s >>= k_s)
-      (st_t, UpdateProph pre_t post_t arg_t >>= k_t).
+      (st_s, FRPrePost pre_s post_s >>= k_s)
+      (st_t, FRPrePost pre_t post_t >>= k_t).
   Proof.
     iIntros "H".
-    rewrite /UpdateProph; unseal CRIS_PROPH.
+    rewrite /FRPrePost; unseal CRIS_FancyReal.
     norm_r; iApply isim_choose_tgt; iIntros (pr).
-    norm_r; iApply isim_choose_tgt; iIntros (ret).
     norm_r; iApply isim_guarantee_tgt; iIntros "P".
-    iPoseProof ("H" $! ret (Own pr) with "[] P") as "[% [% [[% #Hprecise] [Hsplit Hrest]]]]".
+    iPoseProof ("H" $! (Own pr) with "[] P") as "[% [[% #Hprecise] [Hsplit Hrest]]]".
     { iApply precise_Own. }
-    do 2 (norm_l; iApply isim_choose_src; iExists _).
+    norm_l; iApply isim_choose_src; iExists _.
     norm_l; iApply isim_guarantee_src; iSplitL "Hsplit".
     { iIntros "% P"; iMod ("Hsplit" with "P") as "[P $]".
       iDestruct "Hprecise" as "[? H]"; iApply "H"; done.
@@ -931,7 +928,7 @@ Section Proph.
     norm_r; iApply isim_assume_res_tgt; iFrame "P".
     norm_l; norm_r; done.
   Qed.
-End Proph.
+End FancyReal.
 
 Section FSEM.
   Context `{_crisG: !crisG Γ Σ α β τ _S _I}.  
